Prove completeness by cheating: add bind and fmap as constructor in ctxr
The reason for this "cheat" is that, in the proof of completeness, given
any arbitrary V, we may not be able to construct ctxr V \empty to instantiate
the hypothesis. We need the two "cheating" constructor to get around this
issue.

ctx-equiv-ixfree/lang.v
@@ -146,9 +146,9 @@ Qed.
 (** Outside-in evaluation contexts, similar to a normal list *)
 
 Inductive rctx (V : Set) :=
-  | rctx_hole
-  | rctx_app1 (R : rctx V) (e : expr V)
-  | rctx_app2 (v : val V) (R : rctx V).
+| rctx_hole
+| rctx_app1 (R : rctx V) (e : expr V)
+| rctx_app2 (v : val V) (R : rctx V).
 
 Arguments rctx_hole {V}.
 Arguments rctx_app1 {V} R e.
@@ -319,11 +319,11 @@ Proof.
   exact (rctx_ectx_bijection_aux ectx_hole R).
 Qed.
 
-Lemma plug_rplug_equiv {V} (E : ectx V) (e : expr V) :
-  plug E e = rplug (ectx_to_rctx E) e.
+Lemma ectx_to_rctx_correct {V} (E : ectx V) (e : expr V) :
+  rplug (ectx_to_rctx E) e = plug E e.
 Proof.
   unfold ectx_to_rctx.
-  rewrite -> ectx_comp_rctx2_correct. simpl. reflexivity.
+  exact (ectx_comp_rctx2_correct E rctx_hole e).
 Qed.
 
 Lemma plug_eq_val_inv {V} E e (v : val V) :
@@ -686,8 +686,8 @@ Lemma unique_decomposition {V} (E1 E2 : ectx V) e1 e2 :
   E1 = E2 ∧ e1 = e2.
 Proof.
   intros He1 He2 Heq.
-  rewrite -> plug_rplug_equiv in Heq.
-  rewrite -> plug_rplug_equiv in Heq.
+  rewrite <- ectx_to_rctx_correct in Heq.
+  rewrite <- ectx_to_rctx_correct in Heq.
   destruct (unique_rdecomposition _ _ _ _ He1 He2 Heq) as [Heq1 Heq2].
   split.
   - rewrite <- (ectx_rctx_bijection E1).
@@ -1332,6 +1332,8 @@ Qed.
 (** General program contexts *)
 Inductive ctx : Set → Type :=
 | ctx_hole : ctx ∅
+| ctx_fmap {A B} : (A [→] B) → ctx B → ctx A
+| ctx_bind {A B} : (A [⇒] B) → ctx B → ctx A
 | ctx_lam {V} : ctx V → ctx (inc V)
 | ctx_app1 {V} : ctx V → expr V → ctx V
 | ctx_app2 {V} : expr V → ctx V → ctx V.
@@ -1340,6 +1342,8 @@ Inductive ctx : Set → Type :=
 Fixpoint ciplug {V} (C : ctx V) : expr V → expr ∅ :=
   match C with
   | ctx_hole => λ e, e
+  | ctx_fmap f C => λ e, ciplug C (fmap f e)
+  | ctx_bind f C => λ e, ciplug C (bind f e)
   | ctx_lam C => λ e, ciplug C (v_lambda e)
   | ctx_app1 C e2 => λ e, ciplug C (app e e2)
   | ctx_app2 e1 C => λ e, ciplug C (app e1 e)
@@ -1347,6 +1351,8 @@ Fixpoint ciplug {V} (C : ctx V) : expr V → expr ∅ :=
 
 Inductive ctxr : Set → Set → Type :=
 | ctxr_hole {A} : ctxr A A
+| ctxr_fmap {A B C} : (A [→] B) → ctxr B C → ctxr A C
+| ctxr_bind {A B C} : (A [⇒] B) → ctxr B C → ctxr A C
 | ctxr_lam {A B} : ctxr A (inc B) → ctxr A B
 | ctxr_app1 {A B} : ctxr A B → expr B → ctxr A B
 | ctxr_app2 {A B} : expr B → ctxr A B → ctxr A B.
@@ -1355,6 +1361,8 @@ Inductive ctxr : Set → Set → Type :=
 Fixpoint crplug {A B} (C : ctxr A B) : expr A → expr B :=
   match C with
   | ctxr_hole => λ e, e
+  | ctxr_fmap f C => λ e, crplug C (fmap f e)
+  | ctxr_bind f C => λ e, crplug C (bind f e)
   | ctxr_lam C => λ e, v_lambda (crplug C e)
   | ctxr_app1 C e2 => λ e, app (crplug C e) e2
   | ctxr_app2 e1 C => λ e, app e1 (crplug C e)
@@ -1788,6 +1796,36 @@ Proof.
   apply E_rel_o_elimE; assumption.
 Qed.
 
+Lemma compat_fmap {A B} (f : A [→] B) e1 e2 n :
+  n ⊨ E_rel_o e1 e2 →
+  n ⊨ E_rel_o (fmap f e1) (fmap f e2).
+Proof.
+  intros He.
+  apply E_rel_o_intro. iintros γ1 γ2 Hγ.
+  rewrite -> (map_to_bind f).
+  rewrite -> (map_to_bind f).
+  rewrite -> bind_bind_comp'.
+  rewrite -> bind_bind_comp'.
+  apply E_rel_o_elimE. exact He.
+  apply G_rel_intro. iintros x. term_simpl.
+  apply G_rel_elimV. exact Hγ.
+Qed.
+
+Lemma compat_bind {A B} (f : A [⇒] B) e1 e2 n :
+  n ⊨ E_rel_o e1 e2 →
+  n ⊨ E_rel_o (bind f e1) (bind f e2).
+Proof.
+  intros He.
+  apply E_rel_o_intro. iintros γ1 γ2 Hγ.
+  rewrite -> bind_bind_comp'.
+  rewrite -> bind_bind_comp'.
+  apply E_rel_o_elimE. exact He.
+  apply G_rel_intro. iintros x. term_simpl.
+  apply V_rel_o_elimV.
+  - apply fundamental_property_v.
+  - exact Hγ.
+Qed.
+
 Lemma precongruence {A B} (e1 e2 : expr A) (C : ctxr A B) n :
   n ⊨ E_rel_o e1 e2 →
   n ⊨ E_rel_o (cplug C e1) (cplug C e2).
@@ -1795,6 +1833,8 @@ Proof.
   intros He.
   induction C; simpl.
   - exact He.
+  - apply IHC. apply compat_fmap. exact He.
+  - apply IHC. apply compat_bind. exact He.
   - apply compat_val.
     apply compat_lambda.
     apply IHC. exact He.
@@ -1928,6 +1968,42 @@ Proof.
   rewrite <- (bind_pure' (cplug C e2)).
   apply O_rel_o_elimO. exact He.
   apply G_rel_intro. iintros x. destruct x.
+Qed.
+
+(*
+Theorem ciu_equiv_soundness {V} (e1 e2 : expr V) :
+  ciu_equiv e1 e2 →
+  ctx_equiv e1 e2.
+Proof.
+Abort.
+*)
+
+Fixpoint rctx_to_ctxr {V} (R : rctx V) : ctxr V V :=
+  match R with
+  | rctx_hole => ctxr_hole
+  | rctx_app1 R e => ctxr_app1 (rctx_to_ctxr R) e
+  | rctx_app2 v R => ctxr_app2 v (rctx_to_ctxr R)
+  end.
+
+Lemma rctx_to_ctxr_correct {V} (R : rctx V) (e : expr V) :
+  crplug (rctx_to_ctxr R) e = rplug R e.
+Proof.
+  induction R.
+  - simpl. reflexivity.
+  - simpl. rewrite -> IHR. reflexivity.
+  - simpl. rewrite -> IHR. reflexivity.
+Qed.
+
+Theorem ciu_equiv_completeness {V} (e1 e2 : expr V) :
+  ctx_equiv e1 e2 →
+  ciu_equiv e1 e2.
+Proof.
+  unfold ctx_equiv, ciu_equiv.
+  intros He E γ.
+  rewrite <-2 ectx_to_rctx_correct.
+  rewrite <-2 rctx_to_ctxr_correct.
+  specialize (He (ctxr_bind γ (rctx_to_ctxr (ectx_to_rctx E)))).
+  simpl in He. exact He.
 Qed.
 
 (*
